Few nits, and remove redundant stack_ in stack.v.

stack.v
@@ -4,95 +4,95 @@ Require Import Coq.Lists.List.
 Import ListNotations.
 
 Module Stack.
-  (* TODO: stack_equiv showing empty and singleton tuples can be reduced *)
+  (* TODO: equiv showing empty and singleton tuples can be reduced *)
   Inductive Stack: Set :=
   | snil
   | snat (n: nat) (s: Stack)
   | stuple (t: Stack) (s: Stack).
 
-  Function stack_prefix (n: nat) (s: Stack): option Stack :=
+  Function prefix (n: nat) (s: Stack): option Stack :=
     match n with
     | 0 => Some snil
     | S n' =>
       match s with
       | snil => None
       | snat m s =>
-        match stack_prefix n' s with
+        match prefix n' s with
         | None => None
         | Some s' => Some (snat m s')
         end
       | stuple t s =>
-        match stack_prefix n' s with
+        match prefix n' s with
         | None => None
         | Some s' => Some (stuple t s')
         end
       end
     end.
 
-  Function stack_postfix (n: nat) (s: Stack): option Stack :=
+  Function postfix (n: nat) (s: Stack): option Stack :=
     match n with
     | 0 => Some s
     | S n' =>
       match s with
       | snil => None
       | snat _ s'
-      | stuple _ s' => stack_postfix n' s'
+      | stuple _ s' => postfix n' s'
       end
     end.
 
-  Function stack_append (s1 s2: Stack): Stack :=
+  Function append (s1 s2: Stack): Stack :=
     match s1 with
     | snil => s2
-    | snat n s => snat n (stack_append s s2)
-    | stuple t s => stuple t (stack_append s s2)
+    | snat n s => snat n (append s s2)
+    | stuple t s => stuple t (append s s2)
     end.
 
-  Function stack_del (n: nat) (s: Stack): option Stack :=
+  Function del (n: nat) (s: Stack): option Stack :=
     match (s, n) with
     | (snil, _) => None
     | (snat _ s, 0)
     | (stuple _ s, 0) => Some s
     | (snat m s, S n) =>
-      match stack_del n s with
+      match del n s with
       | None => None
       | Some s' => Some (snat m s')
       end
     | (stuple t s, S n) =>
-      match stack_del n s with
+      match del n s with
       | None => None
       | Some s' => Some (stuple t s')
       end
     end.
 
-  Function stack_get (n: nat) (s: Stack): option Stack :=
-    match stack_postfix n s with
+  Function get (n: nat) (s: Stack): option Stack :=
+    match postfix n s with
     | None | Some snil => None
     | Some (snat m _) => Some (snat m s)
     | Some (stuple t _) => Some (stuple t s)
     end.
 
-  Example stack_prefix_ex:
-    forall s, stack_prefix 1 (snat 3 s) = Some (snat 3 snil).
+  Example prefix_ex:
+    forall s, prefix 1 (snat 3 s) = Some (snat 3 snil).
   Proof. intros; auto. Qed.
 
-  Function stack_pack (n: nat) (s: Stack): option Stack :=
+  Function pack (n: nat) (s: Stack): option Stack :=
     match n with
     | 0 | 1 => Some s
     | _ =>
-      match (stack_prefix n s, stack_postfix n s) with
+      match (prefix n s, postfix n s) with
       | (Some t, Some s') => Some (stuple t s')
       | _ => None
       end
     end.
 
-  Example stack_pack_simple:
-    stack_pack 2 (snat 0 (snat 1 snil)) =
+  Example pack_simple:
+    pack 2 (snat 0 (snat 1 snil)) =
     Some (stuple (snat 0 (snat 1 snil)) snil).
   Proof. auto. Qed.
 
-  Example stack_pack_nested:
+  Example pack_nested:
     forall tl,
-      stack_pack 3 (snat 1
+      pack 3 (snat 1
                          (stuple (snat 2 (snat 3 snil))
                                  (snat 4 tl))) =
       Some (stuple (snat 1
@@ -101,43 +101,42 @@ Module Stack.
                    tl).
   Proof. intros; auto. Qed.
 
-  Function stack_unpack (s: Stack): option Stack :=
+  Function unpack (s: Stack): option Stack :=
     match s with
     | snil => None
     | snat _ _ => Some s
-    | stuple t s => Some (stack_append t s)
+    | stuple t s => Some (append t s)
     end.
-    
-  Function stack_cond_get (stack : Stack) (n : nat) (k : nat) :=
+
+  Function cond_get (stack : Stack) (n : nat) (k : nat) :=
     match stack with
-    | Stack.snat 0 _ => Stack.stack_get n stack
-    | Stack.snat _ _ => Stack.stack_get k stack
+    | Stack.snat 0 _ => Stack.get n stack
+    | Stack.snat _ _ => Stack.get k stack
     | _ => None
     end.
 
-  Function stack_weight (s: Stack): nat :=
+  Function weight (s: Stack): nat :=
     match s with
     | snil => 0
-    | snat _ s' => S (stack_weight s')
-    | stuple t s' => S (stack_weight t + stack_weight s')
+    | snat _ s' => S (weight s')
+    | stuple t s' => S (weight t + weight s')
     end.
 
-  Function stack_inc (s: Stack): option Stack :=
+  Function inc (s: Stack): option Stack :=
     match s with
     | snat m s' => Some (snat (S m) s')
     | _ => None
     end.
 
-  Function stack_dec (s: Stack): option Stack :=
+  Function dec (s: Stack): option Stack :=
     match s with
     | snat m s' => Some (snat (pred m) s')
     | _ => None
     end.
 
-  Function stack_out (s: Stack): (option nat) :=
+  Function out (s: Stack): (option nat) :=
     match s with
     | snat m s' => Some m
     | _ => None
     end.
-
 End Stack.
